src/utils/utils.py
@@ -92,12 +92,16 @@ def parse_data_to_dict(data):
     return parsed_data
 
 
-def get_examples_db_task_id_des_pair(example_json):
+def get_examples_db_task_id_spec_pair(example_json):
     list_of_examples = []
     for t in example_json:
         output_task = {
             "task_id": example_json[t]["task_id"],
-            "task_description": example_json[t]["task_description"]
+            "task_description": example_json[t]["task_description"],
+            "api_with_preconditions": example_json[t]["api_with_preconditions"],
+            # "safety_properties": example_json[t]["safety_properties"],
+            # "verification_methods_signature": example_json[t]["spec"]["verification_methods_signature"],
+            # "verification_conditions": example_json[t]["spec"]["verification_conditions"],
         }
         list_of_examples.append(output_task)
     return list_of_examples
@@ -106,14 +110,15 @@ def get_examples_db_task_id_des_pair(example_json):
 def get_examples_id_task_specification_pair(example_json):
     list_of_examples = []
     for task in example_json:
-        print(f"example_json[task]: {example_json[task]}")
+        # print(f"example_json[task]: {example_json[task]}")
         output_task = {
-            "task_id": example_json[task]["task_id"],
-            "task_description": example_json[task]["task_description"],
-            "method_signature": example_json[task]["method_signature"],
-            "safety_properties": example_json[task]["safety_properties"],
-            "verification_methods_signature": example_json[task]["spec"]["verification_methods_signature"],
-            "verification_conditions": example_json[task]["spec"]["verification_conditions"],
+            "task_id": example_json[task]['task_id'],
+            "task_description": example_json[task]['task_description'],
+            "method_signature": example_json[task]['method_signature'],
+            "api_with_preconditions": example_json[task]['api_with_preconditions'],
+            # "safety_properties": example_json[task]["safety_properties"],
+            # "verification_methods_signature": example_json[task]["spec"]["verification_methods_signature"],
+            # "verification_conditions": example_json[task]["spec"]["verification_conditions"],
         }
         list_of_examples.append(output_task)
     return list_of_examples
@@ -136,6 +141,19 @@ def get_examples_id_task_specification_pair(example_json):
     #             })
     #     list_of_examples.append(output_task)
     # return list_of_examples
+
+def get_vc_methods_sp_pair(example_json):
+    list_of_vc_methods = []
+    for t in example_json:
+        print(f"example_json[t]: {example_json[t]}")
+        output_task = {
+            "sp_id": example_json[t]["sp_id"],
+            "safety_property": example_json[t]["safety_property"],
+            "verification_methods_signature": example_json[t]["verification_methods_signature"],
+            "verification_method_description": example_json[t]["verification_method_description"]
+        }
+        list_of_vc_methods.append(output_task)
+    return list_of_vc_methods
 
 def save_to_json(map, file_path):
     json_string = json.dumps(map)
@@ -167,12 +185,8 @@ def prepend_include_to_code(response, interface_path):
     pattern = r'```dafny\n(.*?)```'
     dafny_blocks = re.findall(pattern, response, re.DOTALL)
     for block in dafny_blocks:
-        print(f" ----------------------------- \n\n\n")
-        print(f"block: {block}")
-        modified_block = f'include "{interface_path}"\n\n{block.strip()}'
-        
+        modified_block = f'include "{interface_path}"\n\n{block.strip()}'  
         response = response.replace(f'```dafny\n{block}```', 
                                                       f'```dafny\n{modified_block}\n```')
         
-    print(f" included \n\n\n\n\n\ {response}")
     return response
