dataset/cwe-samples/RAG_samples/task_id_4.dfy
@@ -1,0 +1,29 @@
+include "/Users/pari/pcc-llms/dataset/filesystems/interface/effectful-interface.dfy"
+method Copy(srcFile: seq<char>, dstFile: seq<char>)
+requires is_valid_path_name(srcFile)
+requires is_valid_path_name(dstFile)
+requires non_empty_string(srcFile)
+requires non_empty_string(dstFile)
+requires is_valid_file_extension(srcFile)
+requires is_valid_file_extension(dstFile)
+requires !has_dangerous_pattern(srcFile)
+requires !has_dangerous_pattern(dstFile)
+requires has_valid_path_length(srcFile)
+requires has_valid_path_length(dstFile)
+requires is_valid_file_extension(srcFile)
+requires is_valid_file_extension(dstFile)
+{
+  var f: FileStream;
+  var ok: bool;
+  ok, f := FileStream.Open(srcFile);
+  if !ok { 
+    print "open failed"; 
+    return; 
+  }
+  var data := new byte[100];
+  var dataLength: int32 := 100; 
+  ok := f.Read(srcFile, 0, data, 0, dataLength);
+  ok, f:= FileStream.Open(dstFile);
+    if !ok { print "open failed"; return; }
+  ok := f.Write(dstFile, 0, data, 0, data.Length as int32);
+}
